Link: [[Proof#Proof by induction]]
## 1

![[Pasted image 20241114010554.png|left|500]]

1. {i} **Base**
	1. By definition of addition know 0+0 = 0
	2. By definition of multiplication know 2x0 = 0
	3. From 1) and 2) it follows that 0+0 = 2x0
2. **Induction step**: show (k+1) + (k+1) = 2(k+1)
	1. By def of addition know $(k+1) + (k+1) = (k+k) + (1+1)$
	2. By induction hypothesis
	3. by def of + 
	4. by def of + and *

## 2

![[Pasted image 20241114014052.png|left|400]]

1. {i} Property is $3\times (n+2) = (3\times n) + 6$
2. **Base:** Let n=0. Show $3\times (0+2) = (3\times0) + 6$ holds.
	1. By definition of multiplication and addition know $3\times (0+2) = 6$
	2. By definition of multiplication and addition know $(3*0) + 6 = 6$
	3. From 1) and 2) know $3\times (0+2) = (3\times0) + 6$
3. **Induction Step:** Let $k\in \Bbb N$
	1. Assume $3\times (k+2) = (3\times k) + 6$ holds. (Induction hypothesis)
	2. Show $3\times ((k+1)+2) = (3\times (k+1)) + 6$ holds.
4. ...
	1. By definition of addition know $3\times ((k+1)+2) = 3\times ((k+2)+1)$.
	2. By definition of addition and multiplication know $3\times ((k+2)+1) = 3(k+2) + 3\times 1$
	3. By induction hypothesis know $3(k+2) + 3\times 1 = (3k) + 6 + 3\times 1$
	4. By definition of + and $\times$ know that $(3k)+6+3\times 1 = 1$